CtrlPlaneInvariants.v
@@ -1,0 +1,94 @@
+(* Various helper lemmas showing ctrl plane maps don't change *)
+From MyProject Require Import CrTransformer.
+From MyProject Require Import CrIdentifiers.
+From MyProject Require Import CrConcreteSemantics.
+From MyProject Require Import SmtExpr.
+From MyProject Require Import CrSymbolicSemantics.
+Require Import Coq.Lists.List.
+
+(* Effectively, ctrl plane doesn't change *)
+Lemma ctrl_plane_invariant_hdr_op:
+  forall (ho: HdrOp)
+         (c1: ProgramState uint8),
+  ctrl_plane_map (eval_hdr_op_assign_uint8 ho c1) =
+  ctrl_plane_map c1.
+Proof.
+  intros ho c1.
+  destruct ho; simpl; try reflexivity.
+Qed.
+
+(* Effectively, ctrl plane doesn't change *)
+Lemma ctrl_plane_invariant_hdr_op_list:
+  forall hol c1,
+  ctrl_plane_map (eval_hdr_op_list_uint8 hol c1) =
+  ctrl_plane_map c1.
+Proof.
+  intros.
+  induction hol.
+  - reflexivity.
+  - simpl. rewrite <- IHhol.
+    apply ctrl_plane_invariant_hdr_op.
+Qed.
+
+
+Lemma ctrl_plane_invariant_seq_rule:
+  forall s c,
+    ctrl_plane_map (eval_seq_rule_uint8 s c) =
+    ctrl_plane_map c.
+Proof.
+  intros.
+  unfold eval_seq_rule_uint8.
+  destruct s.
+  destruct (eval_match_uint8 match_pattern c).
+  apply ctrl_plane_invariant_hdr_op_list.
+  reflexivity.
+Qed.
+
+Lemma ctrl_plane_invariant_par_rule:
+  forall p c,
+    ctrl_plane_map (eval_par_rule_uint8 p c) =
+    ctrl_plane_map c.
+Proof.
+  intros.
+  unfold eval_par_rule_uint8.
+  destruct p.
+  destruct (eval_match_uint8 match_pattern c).
+  apply ctrl_plane_invariant_hdr_op_list.
+  reflexivity.
+Qed.
+
+Lemma ctrl_plane_invariant_ma_rule:
+  forall m c,
+    ctrl_plane_map (eval_match_action_rule_uint8 m c) =
+    ctrl_plane_map c.
+Proof.
+  intros.
+  unfold eval_match_action_rule_uint8.
+  destruct m.
+  - apply ctrl_plane_invariant_seq_rule.
+  - apply ctrl_plane_invariant_par_rule.
+Qed.
+
+Lemma ctrl_plane_invariant_transformer_intermediate:
+  forall a t c,
+    ctrl_plane_map (eval_transformer_uint8 (a :: t) c) =
+    ctrl_plane_map (eval_transformer_uint8 t c).
+Proof.
+  intros.
+  unfold eval_transformer_uint8.
+  remember (a :: t) as full_list.
+  remember (find_first_match (combine (get_match_results full_list c) full_list)) as outer_match.
+  remember (find_first_match (combine (get_match_results t c) t)) as inner_match.
+  destruct (outer_match) eqn:des; destruct inner_match eqn:des2; try rewrite ctrl_plane_invariant_ma_rule; try reflexivity.
+  rewrite ctrl_plane_invariant_ma_rule. reflexivity.
+Qed.
+
+Lemma ctrl_plane_invariant_transformer:
+  forall c t,
+    ctrl_plane_map (eval_transformer_uint8 t c) = ctrl_plane_map c.
+Proof.
+  intros.
+  induction t.
+  - reflexivity.
+  - rewrite <- IHt. apply ctrl_plane_invariant_transformer_intermediate.
+Qed.
