HelperLemmas.v
@@ -1,0 +1,145 @@
+(* Miscellaneous helper lemmas for ConcreteToSymbolicLemmas.v *)
+From MyProject Require Import CrTransformer.
+From MyProject Require Import CrIdentifiers.
+From MyProject Require Import CrConcreteSemantics.
+From MyProject Require Import SmtExpr.
+Require Import ZArith.
+Require Import Coq.Lists.List.
+From MyProject Require Import CrSymbolicSemantics.
+From Coq Require Import FunctionalExtensionality.
+
+Lemma program_state_equality:
+      forall (ps1 ps2: ProgramState uint8),
+        ctrl_plane_map ps1 = ctrl_plane_map ps2 ->
+        header_map ps1 = header_map ps2 ->
+        state_var_map  ps1 = state_var_map ps2 ->
+        ps1 = ps2.
+Proof.
+  intros ps1 ps2 Hctrl Hhdr Hstate.
+  destruct ps1 as [ctrl1 hdr1 state1].
+  destruct ps2 as [ctrl2 hdr2 state2].
+  simpl in *.
+  f_equal; try assumption.
+Qed.
+
+Lemma program_state_equality_sym:
+      forall (ps1 ps2: ProgramState SmtArithExpr),
+        ctrl_plane_map ps1 = ctrl_plane_map ps2 ->
+        header_map ps1 = header_map ps2 ->
+        state_var_map  ps1 = state_var_map ps2 ->
+        ps1 = ps2.
+Proof.
+  intros ps1 ps2 Hctrl Hhdr Hstate.
+  destruct ps1 as [ctrl1 hdr1 state1].
+  destruct ps2 as [ctrl2 hdr2 state2].
+  simpl in *.
+  f_equal; try assumption.
+Qed.
+
+Lemma nothing_changed_state:
+  forall s f target,
+    eval_sym_state s f = 
+    update_state (eval_sym_state s f) target
+     (eval_smt_arith (state_var_map s target) f).
+Proof.
+  intros s f target.
+  destruct target.
+  unfold eval_sym_state.
+  apply program_state_equality; simpl; try reflexivity.
+  apply functional_extensionality.
+  intros x.
+  destruct x.
+  destruct (uid =? uid0)%positive eqn:des.
+  - apply Pos.eqb_eq in des.
+    rewrite des.
+    reflexivity.
+  - reflexivity.
+Qed.
+
+Lemma nothing_changed_hdr:
+  forall s f target,
+    eval_sym_state s f = 
+    update_hdr (eval_sym_state s f) target
+     (eval_smt_arith (header_map s target) f).
+Proof.
+  intros s f target.
+  destruct target.
+  unfold eval_sym_state.
+  apply program_state_equality; simpl; try reflexivity.
+  apply functional_extensionality.
+  intros x.
+  destruct x.
+  destruct (uid =? uid0)%positive eqn:des.
+  - apply Pos.eqb_eq in des.
+    rewrite des.
+    reflexivity.
+  - reflexivity.
+Qed.
+
+Lemma commute_lookup_eval:
+  forall (s : ProgramState SmtArithExpr) (f : SmtValuation)
+        arg,
+    lookup_uint8 arg (eval_sym_state s f) =
+    eval_smt_arith (lookup_smt arg s) f.
+Proof.
+  intros s f arg.
+  destruct arg; simpl; reflexivity.
+Qed.
+
+
+Lemma find_first_match_lemma:
+  forall {T : Set} (list_of_pair :  list (bool*T)),
+    None = find_first_match list_of_pair ->
+    forall x,
+    In x list_of_pair -> fst x = false.
+Proof.
+  intros.
+  induction list_of_pair as [| [b t] rest].
+  - simpl in H0. contradiction.
+  - simpl in H0. destruct H0 eqn:des.
+    + subst. simpl in H. destruct b.
+      * discriminate H.
+      * reflexivity.
+    + subst. simpl in H. destruct b.
+      * discriminate H.
+      * apply IHrest; assumption.
+Qed.
+
+Lemma find_first_match_lemma2:
+  forall {T : Set} (list_of_pair :  list (bool*T)) element,
+    Some element = find_first_match list_of_pair ->
+    In (true, element) list_of_pair.
+Proof.
+  intros.
+  induction list_of_pair as [| [b t] rest].
+  - simpl in H. discriminate H.
+  - simpl in H.
+    simpl.
+    destruct b.
+    -- inversion H. left. reflexivity.
+    -- right. apply IHrest.
+       assumption.
+Qed.
+
+Lemma header_map_ps :
+  forall s f h,
+    header_map (eval_sym_state s f) h =
+    eval_smt_arith (header_map s h) f.
+Proof.
+  intros.
+  unfold eval_sym_state.
+  simpl.
+  reflexivity.
+Qed.
+
+(* Create a lemma similar to header_map_ps but with state_var_map instead *)
+Lemma state_var_map_ps :
+  forall s f sv,
+    state_var_map (eval_sym_state s f) sv =
+    eval_smt_arith (state_var_map s sv) f.
+Proof.
+  intros.
+  unfold eval_sym_state.
+  simpl.
+  reflexivity.
+Qed.
